General/Lemmas.v
@@ -4,3 +4,13 @@ Lemma not_or_and :
 Proof.
   tauto.
 Qed.
+
+Lemma not_and_or :
+  forall (P Q : Prop),
+  ~P /\ ~Q -> ~(P \/ Q).
+Proof.
+  tauto.
+Qed.
+
+Hint Resolve not_or_and : core.
+Hint Resolve not_and_or : core.
